Refinining JRussell, beginning generation lemmas

proof/JRussell/Coercion.v
@@ -4,9 +4,8 @@ Require Import Lambda.Conv.
 Require Import Lambda.LiftSubst.
 Require Import Lambda.Env.
 Require Import JRussell.Types.
-(*Require Import JRussell.Thinning.
-Require Import JRussell.Substitution.
-*)
+Require Import JRussell.Basic.
+
 Set Implicit Arguments.
 
 Implicit Types i k m n p : nat.
@@ -15,265 +14,123 @@ Implicit Types A B M N T t u v : term.
 Implicit Types e f g : env.
 
 Inductive coerce_in_env : env -> env -> Prop :=
-  | coerce_env_hd : forall e t u s, e |- t >> u : s -> 
-	coerce_in_env (u :: e) (t :: e)
+  | coerce_env_hd : forall e t u s, e |- t >> u : s -> e |- u : Srt s -> 
+	coerce_in_env (t :: e) (u :: e)
   | coerce_env_tl :
-        forall e f t, wf (t :: f) -> coerce_in_env e f -> coerce_in_env (t :: e) (t :: f).
+        forall e f t, coerce_in_env e f -> coerce_in_env (t :: e) (t :: f).
 
 Hint Resolve coerce_env_hd coerce_env_tl: coc.
 
-Lemma conv_item :
-   forall n t e,
-   item_lift t e n ->
-   forall f, coerce_in_env e f ->
-   item_lift t f n \/
-   ((forall g, trunc _ (S n) e g -> trunc _ (S n) f g) /\
-   exists u, item_lift u f n /\ (exists s, f |- u >> t : s)).
-simple induction n.
-do 3 intro.
-elim H.
-do 4 intro.
-rewrite H0.
-inversion_clear H1.
-intros.
-inversion_clear H1.
-right.
-split; intros.
-inversion_clear H1; auto with coc core arith datatypes.
-
-exists (lift 1 t0).
-split.
-inversion_clear H.
-
-unfold item_lift.
-exists t0; auto with coc core arith datatypes.
-
-exists s ; auto with coc core.
-apply thinning_n_coerce with l ; auto with coc core.
-apply wf_var with s.
-apply coerce_sort_l with x ; auto with coc.
-
-left.
-exists x; auto with coc core arith datatypes.
-
-do 5 intro.
-elim H0.
-do 4 intro.
-rewrite H1.
-inversion_clear H2.
-intros.
-inversion_clear H2.
-left.
-exists x; auto with coc core arith datatypes.
-
-elim H with (lift (S n0) x) l f0; auto with coc core arith datatypes; intros.
-left.
-elim H2; intros.
-exists x0; auto with coc core arith datatypes.
-rewrite simpl_lift.
-pattern (lift (S (S n0)) x0) in |- *.
-rewrite simpl_lift.
-elim H6; auto with coc core arith datatypes.
-
-right.
-elim H2.
-clear H2.
-simple induction 2; intros.
-clear H6.
-split; intros.
-inversion_clear H6; auto with coc core arith datatypes.
-
-destruct H7.
-destruct H7.
-unfold item_lift.
-exists (lift 1 x0).
-split ; auto with coc core.
-inversion_clear H6 ; auto with coc core arith.
-exists x2.
-rewrite H8.
-rewrite <- simpl_lift.
-auto with coc core.
-auto with coc.
-
-exists x1.
-pattern (lift (S (S n0)) x) ; rewrite simpl_lift.
-eapply thinning_n_coerce ; auto with coc core.
-
-exists x; auto with coc core arith datatypes.
-Qed.
-
-Lemma double_conv_env :
+Lemma ind_coerce_env :
   (forall e t T, e |- t : T -> 
-  forall f, coerce_in_env e f -> 
-  wf f -> f |- t : T) /\
+  forall f, coerce_in_env e f -> f |- t : T) /\
   (forall e T U s, e |- T >> U : s -> 
-  forall f, coerce_in_env e f -> 
-  wf f -> f |- T >> U : s).
+  forall f, coerce_in_env e f -> f |- T >> U : s) /\
+  (forall e U V T, e |- U = V : T ->
+  forall f, coerce_in_env e f -> f |- U = V : T).
 Proof.
-apply double_typ_coerce_mut with 
+apply typ_coerce_jeq_ind with 
 (P := fun e t T => fun H : typ e t T =>
   forall f, coerce_in_env e f -> 
-  wf f -> typ f t T)
+  typ f t T)
 (P0 := fun e T U s => fun H : e |- T >> U : s =>
   forall f, coerce_in_env e f -> 
-  wf f -> f |- T >> U : s) ; intros ;
+  f |- T >> U : s) 
+(P1 := fun e U V T => fun H : e |- U = V : T =>
+  forall f, coerce_in_env e f -> 
+  f |- U = V : T) ;
+ intros ; try (solve [destruct (H f H0) ; clear H]); 
 auto with coc core arith datatypes.
 
-elim conv_item with n T e f; auto with coc core arith datatypes; intros.
-repeat destruct H1.
-destruct H2.
-destruct H2.
-destruct H3.
-destruct (coerce_sort H3).
-apply type_conv with x x0 ; auto with coc core.
+inversion H ; auto with coc.
+inversion H ; auto with coc.
 
-cut (wf (T :: f)); intros.
-apply type_abs with s1 s2; auto with coc core arith datatypes.
-apply wf_var with s1; auto with coc core arith datatypes.
+inversion H0.
+apply type_conv with (lift 1 u) s0 ; auto with coc.
+apply type_var with s0 ; auto with coc .
+apply coerce_weak with s0 ; auto with coc.
 
-apply type_app with V; auto with coc core arith datatypes.
+apply type_var with s ; auto with coc.
 
-cut (wf (U :: f)); intros.
-apply type_pair with s1 s2 s3; auto with coc core arith datatypes.
-apply wf_var with s1 ; auto with coc core.
+inversion H1.
+apply type_weak with s0 ; auto.
+apply type_weak with s ; auto.
 
-cut (wf (T :: f)); intros.
-apply type_prod with s1; auto with coc core arith datatypes.
+apply type_abs with s1 s2 ; auto with coc.
 
-apply wf_var with s1; auto with coc core arith datatypes.
+apply type_app with V ; auto with coc.
 
-cut (wf (T :: f)); intros.
-apply type_sum with s1 s2; auto with coc core arith datatypes.
+apply type_pair with s1 s2 s3 ; auto with coc.
 
-apply wf_var with s1; auto with coc core arith datatypes.
+apply type_prod with s1 ; auto with coc.
 
-cut (wf (T :: f)); intros.
-apply type_subset; auto with coc core arith datatypes.
+apply type_sum with s1 s2 ; auto with coc.
 
-apply wf_var with set; auto with coc core arith datatypes.
+apply type_subset ; auto with coc.
 
-apply type_pi1 with V ; auto with coc core arith datatypes.
+apply type_pi1 with V ; auto with coc.
 
-apply type_pi2 with U ; auto with coc core arith datatypes.
+apply type_pi2 with U ; auto with coc.
 
-(*cut (wf (U :: f)); intros.
-apply type_let_in with U s1 s2 ; auto with coc core arith datatypes.
-apply wf_var with s1 ; auto with coc core.*)
+apply type_conv with U s ; auto with coc.
 
-apply type_conv with U s; auto with coc core arith datatypes.
+inversion H1.
+apply coerce_weak with s0 ; auto with coc.
+apply coerce_weak with s' ; auto with coc.
 
-cut (wf (A' :: f)) ; intros.
-cut (wf (A :: f)) ; intros.
-apply coerce_prod with s ;auto with coc core arith datatypes.
-apply wf_var with s ; auto with coc core arith datatypes.
-apply wf_var with s ; auto with coc core arith datatypes.
+apply coerce_prod with s ; auto with coc.
 
-cut (wf (A' :: f)) ; intros.
-cut (wf (A :: f)) ; intros.
-apply coerce_sum with s s' ;auto with coc core arith datatypes.
-apply wf_var with s ; auto with coc core arith datatypes.
-apply wf_var with s ; auto with coc core arith datatypes.
+apply coerce_sum with s s' ; auto with coc.
 
-cut (wf (U :: f)) ; intros.
-apply coerce_sub_l ; auto with coc core arith datatypes.
-eapply wf_var ; auto with coc core arith datatypes.
-apply coerce_sort_l with U' ; auto with coc core arith datatypes.
+apply coerce_trans with B ; auto with coc.
 
-cut (wf (U' :: f)) ; intros.
-apply coerce_sub_r ; auto with coc core arith datatypes.
-eapply wf_var ; auto with coc core arith datatypes.
-apply coerce_sort_r with U ; auto with coc core arith datatypes.
+inversion H1.
+apply jeq_weak with s0 ; auto with coc.
+apply jeq_weak with s ; auto with coc.
 
-apply coerce_conv with B C ; auto with coc core arith datatypes.
+apply jeq_prod with s1 ; auto with coc.
+
+apply jeq_abs with s1 s2 ; auto with coc.
+
+apply jeq_app with A ; auto with coc.
+
+apply jeq_beta with s1 s2 ; auto with coc.
+
+apply jeq_red with A s ; auto with coc.
+
+apply jeq_exp with B s ; auto with coc.
+
+apply jeq_sum with s1 s2 ; auto with coc.
+
+apply jeq_pair with s1 s2 s3; auto with coc.
+
+apply jeq_pi1 with B; auto with coc.
+
+apply jeq_pi1_red with s1 s2 s3; auto with coc.
+
+apply jeq_pi2 with A ; auto with coc.
+
+apply jeq_pi2_red with s1 s2 s3; auto with coc.
+
+apply jeq_subset ; auto with coc.
+
+apply jeq_trans with N ; auto with coc.
+
+apply jeq_conv with A s ; auto with coc.
 Qed.
 
-Lemma typ_conv_env : forall e t T, e |- t : T -> forall f, coerce_in_env e f -> 
-  wf f -> f |- t : T.
-Proof (proj1 double_conv_env).
+Lemma typ_coerce_env : forall e t T, e |- t : T -> forall f, coerce_in_env e f -> 
+  f |- t : T.
+Proof (proj1 ind_coerce_env).
 
-Lemma coerce_conv_env : forall e T U s, e |- T >> U : s -> 
+Lemma coerce_coerce_env : forall e T U s, e |- T >> U : s -> 
   forall f, coerce_in_env e f -> 
-  wf f -> f |- T >> U : s.
-Proof (proj2 double_conv_env).
+  f |- T >> U : s.
+Proof (proj1 (proj2 ind_coerce_env)).
 
-Lemma coerce_sym : forall e T U s, e |- T >> U : s -> e |- U >> T : s.
-Proof.
-  intros e T U s H ; induction H ; intros ; auto with coc core.
-  
-  apply coerce_prod with s ; auto with coc.
-  apply coerce_conv_env with (A' :: e) ; auto with coc core arith datatypes.
-  apply coerce_env_hd with s ; auto with coc.
-  apply wf_var with s ; auto with coc.
+Lemma jeq_coerce_env : forall e U V T, e |- U = V : T -> 
+  forall f, coerce_in_env e f -> 
+  f |- U = V : T.
+Proof (proj2 (proj2 ind_coerce_env)).
 
-  apply coerce_sum with s s' ; auto with coc.
-  apply coerce_conv_env with (A :: e) ; auto with coc core arith datatypes.
-  apply coerce_env_hd with s ; auto with coc.
-  apply wf_var with s ; auto with coc.
-
-  apply coerce_conv with C B ; auto with coc core.
-Qed.
-
-Hint Resolve coerce_sym : coc.
-
-(*
-Lemma typ_sort_aux : forall G t T, G |- t : T -> 
-  forall s, t = (Srt s) -> is_prop s /\ T = (Srt kind).
-Proof.
-induction 1 ; intros ; try discriminate.
-
-injection H0 ; intro ; rewrite <- H1 ; unfold is_prop ; intuition.
-
-injection H0 ; intro ; rewrite <- H1 ; unfold is_prop ; intuition.
-
-induction (IHtyp s0 H1).
-split ; auto.
-
-generalize  H0 H3.
-induction 1 ; simpl ; intros ; try discriminate.
-elim typ_not_kind with e A (Srt s) ; auto with coc.
-
-pose (IHcoerce H IHtyp H4 H3 H6).
-rewrite e0 in H0.
-
-
-
-destruct (IHtyp3 _ H5).
-unfold is_prop in H6.
-induction H6 ; discriminate.
-Qed.
-
-Lemma typ_sort : forall G s T, G |- (Srt s) : T -> is_prop s /\ T = (Srt kind).
-Proof.
-intros.
-apply (typ_sort_aux H (refl_equal (Srt s))).
-Qed.
-
-
-Hint Resolve typ_not_kind typ_wf : coc.
-
-Lemma coerce_sort : forall G T U s, 
-  G |- T >> U : s -> (G |- T : Srt s /\ G |- U : Srt s).
-Proof.
-  induction 1 ; intros ; split ; try (intuition ; intros ; auto with coc core).
-  apply type_prod with s ; auto with coc core.
-  apply type_prod with s ; auto with coc core.
-  apply type_sum with s s' ; auto with coc core.
-  apply type_sum with s s' ; auto with coc core.
-  apply type_subset ; auto with coc core.
-  apply type_subset ; auto with coc core.
-Qed.
-
-Lemma coerce_sort_l : forall G T U s, 
-  G |- T >> U : s -> G |- T : Srt s.
-Proof. 
-  intros G T U s H.
-  apply (proj1 (coerce_sort H)).
-Save.
-
-Lemma coerce_sort_r : forall G T U s, 
-  G |- T >> U : s -> G |- U : Srt s.
-Proof. 
-  intros G T U s H.
-  apply (proj2 (coerce_sort  H)).
-Save.
 
