proof/JRussell/Types.v
@@ -19,7 +19,10 @@ Definition sum_sort s1 s2 s3 :=
   (s1 = prop /\ s2 = prop /\ s3 = prop).
 
 Inductive coerce : env -> term -> term -> sort -> Prop :=
-  | coerce_refl : forall e A s, e |- A : Srt s -> e |- A >> A : s
+  | coerce_conv : forall e A B s, e |- A = B : Srt s -> e |- A >> B : s
+  
+  | coerce_weak : forall e A B s, e |- A >> B : s ->
+  forall T s', e |- T : Srt s' -> (T :: e) |- lift 1 A >> lift 1 B : s
 
   | coerce_prod : forall e A B A' B',
   forall s, e |- A' >> A : s ->
@@ -48,12 +51,18 @@ Inductive coerce : env -> term -> term -> sort -> Prop :=
   (* derivable *) U' :: e |- P : Srt prop ->
   e |- U >> (Subset U' P) : set
 
-  | coerce_conv : forall e A B C D s,  
-  e |- A = B : Srt s -> e |- B >> C : s -> e |- C = D : Srt s -> e |- A >> D : s
+  | coerce_sym : forall e U V s, e |- U >> V : s -> e |- V >> U : s
+
+  | coerce_trans : forall e A B C s,  
+  e |- A >> B : s -> e |- B >> C : s -> e |- A >> C : s
 
 where "G |- T >> U : s" := (coerce G T U s)
 
 with jeq : env -> term -> term -> term -> Prop :=
+  | jeq_weak : forall e M N A, e |- M = N : A ->
+  forall B s, e |- B : Srt s ->
+  (B :: e) |- lift 1 M = lift 1 N : lift 1 A
+
   | jeq_prod : forall e U V U' V' s1 s2, 
   e |- U = U' : Srt s1 -> U :: e |- V = V' : Srt s2 ->
   e |- Prod U V = Prod U' V' : Srt s2
@@ -86,29 +95,29 @@ with jeq : env -> term -> term -> term -> Prop :=
   forall s3, sum_sort s1 s2 s3 ->
   e |- Sum A B = Sum A' B' : Srt s3
   
-  | jeq_pi1 : forall e A A' s1, e |- A = A' : Srt s1 ->
+  | jeq_pair : forall e A A' s1, e |- A = A' : Srt s1 ->
   forall B B' s2, (A :: e) |- B = B' : Srt s2 ->
   forall s3, sum_sort s1 s2 s3 ->
-  forall t t', e |- t = t' : Sum A B ->
+  forall u u', e |- u = u' : A ->
+  forall v v', e |- v = v' : subst u B ->
+  e |- Pair (Sum A B) u v = Pair (Sum A' B') u' v' : Sum A B
+
+  | jeq_pi1 : forall e t t' A B, e |- t = t' : Sum A B ->
   e |- Pi1 t = Pi1 t' : A
 
-  | jeq_pi1_red : forall e A A' s1, e |- A = A' : Srt s1 ->
-  forall B B' s2, (A :: e) |- B = B' : Srt s2 ->
+  | jeq_pi1_red : forall e A s1, e |- A : Srt s1 ->
+  forall B s2, (A :: e) |- B : Srt s2 ->
   forall s3, sum_sort s1 s2 s3 ->
-  forall u u' v v', e |- Pair (Sum A B) u v = Pair (Sum A' B') u' v' : Sum A B ->
+  forall u, e |- u : A -> forall v, e |- v : subst u B ->
   e |- Pi1 (Pair (Sum A B) u v) = u : A
 
-  | jeq_pi2 : forall e A A' s1, e |- A = A' : Srt s1 ->
-  forall B B' s2, (A :: e) |- B = B' : Srt s2 ->
-  forall s3, sum_sort s1 s2 s3 ->
-  forall t t', e |- t = t' : Sum A B ->
+  | jeq_pi2 : forall e t t' A B, e |- t = t' : Sum A B ->
   e |- Pi2 t = Pi2 t' : subst (Pi1 t) B
 
-  | jeq_pi2_red : forall e A A' s1, e |- A = A' : Srt s1 ->
-  forall B B' s2, (A :: e) |- B = B' : Srt s2 ->
+  | jeq_pi2_red : forall e A s1, e |- A : Srt s1 ->
+  forall B s2, (A :: e) |- B : Srt s2 ->
   forall s3, sum_sort s1 s2 s3 ->
-  forall u u' v v', 
-  e |- Pair (Sum A B) u v = Pair (Sum A' B') u' v' : Sum A B ->
+  forall u, e |- u : A -> forall v, e |- v : subst u B ->
   e |- Pi2 (Pair (Sum A B) u v) = v : subst u B
 
   | jeq_subset : forall e A A', e |- A = A' : Srt set ->
@@ -121,19 +130,18 @@ with jeq : env -> term -> term -> term -> Prop :=
   
   | jeq_trans : forall e M N P A, e |- M = N : A -> e |- N = P : A -> e |- M =  P : A
   
-  | jeq_conv : forall e M N A B s, e |- M = N : A -> e |- A = B : Srt s -> e |- M = N : B
+  | jeq_conv : forall e M N A B s, e |- M = N : A -> e |- A >> B : s -> e |- M = N : B
 
 where "G |- T = U : s" := (jeq G T U s)
 
-with wf : env -> Prop :=
-  | wf_nil : wf nil
-  | wf_var : forall e T s, e |- T : (Srt s) -> wf (T :: e)
-
 with typ : env -> term -> term -> Prop :=
-  | type_prop : forall e, wf e -> e |- (Srt prop) : (Srt kind)
-  | type_set : forall e, wf e -> e |- (Srt set) : (Srt kind)	
-  | type_var : (* start *)
-      forall e, wf e -> forall n T, item_lift T e n -> e |- (Ref n) : T
+  | type_prop : nil |- (Srt prop) : (Srt kind)
+  | type_set : nil |- (Srt set) : (Srt kind)	
+  | type_var :
+      forall e T s, e |- T : Srt s -> (T :: e) |- (Ref 0) : (lift 1 T)
+  | type_weak :
+      forall e t T, e |- t : T -> forall U s, e |- U : Srt s ->
+      (U :: e) |- lift 1 t : lift 1 T
   | type_abs :
       forall e T s1,
       e |- T : (Srt s1) ->
@@ -190,23 +198,15 @@ with typ : env -> term -> term -> Prop :=
 
 where "G |- T : U" :=  (typ G T U).
 
-Hint Resolve coerce_refl coerce_conv coerce_prod coerce_sum coerce_sub_l coerce_sub_r : coc.
+Hint Resolve coerce_conv coerce_weak coerce_sym coerce_prod coerce_sum coerce_sub_l coerce_sub_r coerce_trans : coc.
 Hint Resolve jeq_refl jeq_sym jeq_beta : coc.
-Hint Resolve type_pi1 type_pi2 type_pair type_prop type_set type_var: coc.
+Hint Resolve type_pi1 type_pi2 type_pair type_prop type_set type_var type_weak: coc.
 
 Scheme typ_dep := Induction for typ Sort Prop.
-
-Scheme typ_wf_mut := Induction for typ Sort Prop
-with wf_typ_mut := Induction for wf Sort Prop.
 
 Scheme typ_coerce_jeq_mutind := Induction for typ Sort Prop
 with coerce_typ_jeq_mutind := Induction for coerce Sort Prop
 with jeq_typ_coerce_mutind := Induction for jeq Sort Prop.
-
-Scheme typ_coerce_wf_jeq_mutind := Induction for typ Sort Prop
-with coerce_typ_wf_jeq_mutind := Induction for coerce Sort Prop
-with jeq_typ_wf_coerce_mutind := Induction for jeq Sort Prop
-with wf_typ_coerce_jeq_mutind := Induction for wf Sort Prop.
 
 Check typ_coerce_jeq_mutind.
 
@@ -214,10 +214,15 @@ Lemma typ_coerce_jeq_ind :
 forall (P : forall (e : env) t t0, e |- t : t0 -> Prop)
          (P0 : forall (e : env) t t0 s, e |- t >> t0 : s -> Prop)
          (P1 : forall (e : env) t t0 t1, e |- t = t0 : t1 -> Prop),
-       (forall (e : env) (w : wf e), P e (Srt prop) (Srt kind) (type_prop w)) ->
-       (forall (e : env) (w : wf e), P e (Srt set) (Srt kind) (type_set w)) ->
-       (forall (e : env) (w : wf e) n T (i : item_lift T e n),
-        P e (Ref n) T (type_var w i)) ->
+       P nil (Srt prop) (Srt kind) type_prop ->
+       P nil (Srt set) (Srt kind) type_set ->
+       (forall (e : env) T s (t : e |- T : Srt s),
+        P e T (Srt s) t -> P (T :: e) (Ref 0) (lift 1 T) (type_var t)) ->
+       (forall (e : env) t T (t0 : e |- t : T),
+        P e t T t0 ->
+        forall (U : term) s (t1 : e |- U : Srt s),
+        P e U (Srt s) t1 ->
+        P (U :: e) (lift 1 t) (lift 1 T) (type_weak t0 t1)) ->
        (forall (e : env) T s1 (t : e |- T : Srt s1),
         P e T (Srt s1) t ->
         forall M (U : term) s2 (t0 : T :: e |- U : Srt s2),
@@ -261,8 +266,13 @@ forall (P : forall (e : env) t t0, e |- t : t0 -> Prop)
         P e t U t0 ->
         forall s (c : e |- U >> V : s),
         P0 e U V s c -> P e t V (type_conv t0 c)) ->
-       (forall (e : env) A s (t : e |- A : Srt s),
-        P e A (Srt s) t -> P0 e A A s (coerce_refl t)) ->
+       (forall (e : env) A B s (j : e |- A = B : Srt s),
+        P1 e A B (Srt s) j -> P0 e A B s (coerce_conv j)) ->
+       (forall (e : env) A B s (c : e |- A >> B : s),
+        P0 e A B s c ->
+        forall T s' (t : e |- T : Srt s'),
+        P e T (Srt s') t ->
+        P0 (T :: e) (lift 1 A) (lift 1 B) s (coerce_weak c t)) ->
        (forall (e : env) A B A' B' s (c : e |- A' >> A : s),
         P0 e A' A s c ->
         forall t : e |- A' : Srt s,
@@ -308,12 +318,17 @@ forall (P : forall (e : env) t t0, e |- t : t0 -> Prop)
         forall t1 : U' :: e |- P2 : Srt prop,
         P (U' :: e) P2 (Srt prop) t1 ->
         P0 e U (Subset U' P2) set (coerce_sub_r c t t0 t1)) ->
-       (forall (e : env) A B (C D : term) s (j : e |- A = B : Srt s),
-        P1 e A B (Srt s) j ->
-        forall c : e |- B >> C : s,
-        P0 e B C s c ->
-        forall j0 : e |- C = D : Srt s,
-        P1 e C D (Srt s) j0 -> P0 e A D s (coerce_conv j c j0)) ->
+       (forall (e : env) (U V : term) s (c : e |- U >> V : s),
+        P0 e U V s c -> P0 e V U s (coerce_sym c)) ->
+       (forall (e : env) A B (C : term) s (c : e |- A >> B : s),
+        P0 e A B s c ->
+        forall c0 : e |- B >> C : s,
+        P0 e B C s c0 -> P0 e A C s (coerce_trans c c0)) ->
+       (forall (e : env) M N A (j : e |- M = N : A),
+        P1 e M N A j ->
+        forall B s (t : e |- B : Srt s),
+        P e B (Srt s) t ->
+        P1 (B :: e) (lift 1 M) (lift 1 N) (lift 1 A) (jeq_weak j t)) ->
        (forall (e : env) (U V U' V' : term) s1 s2 (j : e |- U = U' : Srt s1),
         P1 e U U' (Srt s1) j ->
         forall j0 : U :: e |- V = V' : Srt s2,
@@ -358,31 +373,35 @@ forall (P : forall (e : env) t t0, e |- t : t0 -> Prop)
         P1 e A A' (Srt s1) j ->
         forall B B' s2 (j0 : A :: e |- B = B' : Srt s2),
         P1 (A :: e) B B' (Srt s2) j0 ->
-        forall s3 (s : sum_sort s1 s2 s3) t t' (j1 : e |- t = t' : Sum A B),
-        P1 e t t' (Sum A B) j1 -> P1 e (Pi1 t) (Pi1 t') A (jeq_pi1 j j0 s j1)) ->
-       (forall (e : env) A A' s1 (j : e |- A = A' : Srt s1),
-        P1 e A A' (Srt s1) j ->
-        forall B B' s2 (j0 : A :: e |- B = B' : Srt s2),
-        P1 (A :: e) B B' (Srt s2) j0 ->
-        forall s3 (s : sum_sort s1 s2 s3) u u' v v'
-          (j1 : e |- Pair (Sum A B) u v = Pair (Sum A' B') u' v' : Sum A B),
-        P1 e (Pair (Sum A B) u v) (Pair (Sum A' B') u' v') (Sum A B) j1 ->
-        P1 e (Pi1 (Pair (Sum A B) u v)) u A (jeq_pi1_red j j0 s j1)) ->
-       (forall (e : env) A A' s1 (j : e |- A = A' : Srt s1),
-        P1 e A A' (Srt s1) j ->
-        forall B B' s2 (j0 : A :: e |- B = B' : Srt s2),
-        P1 (A :: e) B B' (Srt s2) j0 ->
-        forall s3 (s : sum_sort s1 s2 s3) t t' (j1 : e |- t = t' : Sum A B),
-        P1 e t t' (Sum A B) j1 ->
-        P1 e (Pi2 t) (Pi2 t') (subst (Pi1 t) B) (jeq_pi2 j j0 s j1)) ->
-       (forall (e : env) A A' s1 (j : e |- A = A' : Srt s1),
-        P1 e A A' (Srt s1) j ->
-        forall B B' s2 (j0 : A :: e |- B = B' : Srt s2),
-        P1 (A :: e) B B' (Srt s2) j0 ->
-        forall s3 (s : sum_sort s1 s2 s3) u u' v v'
-          (j1 : e |- Pair (Sum A B) u v = Pair (Sum A' B') u' v' : Sum A B),
-        P1 e (Pair (Sum A B) u v) (Pair (Sum A' B') u' v') (Sum A B) j1 ->
-        P1 e (Pi2 (Pair (Sum A B) u v)) v (subst u B) (jeq_pi2_red j j0 s j1)) ->
+        forall s3 (s : sum_sort s1 s2 s3) u u' (j1 : e |- u = u' : A),
+        P1 e u u' A j1 ->
+        forall v v' (j2 : e |- v = v' : subst u B),
+        P1 e v v' (subst u B) j2 ->
+        P1 e (Pair (Sum A B) u v) (Pair (Sum A' B') u' v') (Sum A B)
+          (jeq_pair j j0 s j1 j2)) ->
+       (forall (e : env) t t' A B (j : e |- t = t' : Sum A B),
+        P1 e t t' (Sum A B) j -> P1 e (Pi1 t) (Pi1 t') A (jeq_pi1 j)) ->
+       (forall (e : env) A s1 (t : e |- A : Srt s1),
+        P e A (Srt s1) t ->
+        forall B s2 (t0 : A :: e |- B : Srt s2),
+        P (A :: e) B (Srt s2) t0 ->
+        forall s3 (s : sum_sort s1 s2 s3) u (t1 : e |- u : A),
+        P e u A t1 ->
+        forall v (t2 : e |- v : subst u B),
+        P e v (subst u B) t2 ->
+        P1 e (Pi1 (Pair (Sum A B) u v)) u A (jeq_pi1_red t t0 s t1 t2)) ->
+       (forall (e : env) t t' A B (j : e |- t = t' : Sum A B),
+        P1 e t t' (Sum A B) j ->
+        P1 e (Pi2 t) (Pi2 t') (subst (Pi1 t) B) (jeq_pi2 j)) ->
+       (forall (e : env) A s1 (t : e |- A : Srt s1),
+        P e A (Srt s1) t ->
+        forall B s2 (t0 : A :: e |- B : Srt s2),
+        P (A :: e) B (Srt s2) t0 ->
+        forall s3 (s : sum_sort s1 s2 s3) u (t1 : e |- u : A),
+        P e u A t1 ->
+        forall v (t2 : e |- v : subst u B),
+        P e v (subst u B) t2 ->
+        P1 e (Pi2 (Pair (Sum A B) u v)) v (subst u B) (jeq_pi2_red t t0 s t1 t2)) ->
        (forall (e : env) A A' (j : e |- A = A' : Srt set),
         P1 e A A' (Srt set) j ->
         forall B B' (j0 : A :: e |- B = B' : Srt prop),
@@ -398,8 +417,9 @@ forall (P : forall (e : env) t t0, e |- t : t0 -> Prop)
         P1 e N P2 A j0 -> P1 e M P2 A (jeq_trans j j0)) ->
        (forall (e : env) M N A B s (j : e |- M = N : A),
         P1 e M N A j ->
-        forall j0 : e |- A = B : Srt s,
-        P1 e A B (Srt s) j0 -> P1 e M N B (jeq_conv j j0)) ->
+        forall c : e |- A >> B : s, P0 e A B s c -> P1 e M N B (jeq_conv j c)) ->
+
+
        (forall (e : env) t t0 (c : e |- t : t0 ), P e t t0 c)
        /\ (forall (e : env) t t0 s (c : e |- t >> t0 : s), P0 e t t0 s c)
        /\ (forall (e : env) t t0 T (c : e |- t = t0 : T), P1 e t t0 T c).
@@ -412,296 +432,3 @@ Proof.
   eapply jeq_typ_coerce_mutind with (P:=P) (P0:=P0) (P1:=P1) ; auto ; auto.
 Qed.
 
-Check (typ_coerce_wf_jeq_mutind).
-
-Lemma typ_coerce_jeq_wf_ind :
-forall (P : forall (e : env) t t0, e |- t : t0 -> Prop)
-         (P0 : forall (e : env) t t0 s, e |- t >> t0 : s -> Prop)
-         (P1 : forall (e : env) t t0 t1, e |- t = t0 : t1 -> Prop)
-         (P2 : forall e : env, wf e -> Prop),
-       (forall (e : env) (w : wf e),
-        P2 e w -> P e (Srt prop) (Srt kind) (type_prop w)) ->
-       (forall (e : env) (w : wf e),
-        P2 e w -> P e (Srt set) (Srt kind) (type_set w)) ->
-       (forall (e : env) (w : wf e),
-        P2 e w ->
-        forall n T (i : item_lift T e n), P e (Ref n) T (type_var w i)) ->
-       (forall (e : env) T s1 (t : e |- T : Srt s1),
-        P e T (Srt s1) t ->
-        forall M (U : term) s2 (t0 : T :: e |- U : Srt s2),
-        P (T :: e) U (Srt s2) t0 ->
-        forall t1 : T :: e |- M : U,
-        P (T :: e) M U t1 -> P e (Abs T M) (Prod T U) (type_abs t t0 t1)) ->
-       (forall (e : env) v (V : term) (t : e |- v : V),
-        P e v V t ->
-        forall u (Ur : term) (t0 : e |- u : Prod V Ur),
-        P e u (Prod V Ur) t0 -> P e (App u v) (subst v Ur) (type_app t t0)) ->
-       (forall (e : env) (U : term) s1 (t : e |- U : Srt s1),
-        P e U (Srt s1) t ->
-        forall u (t0 : e |- u : U),
-        P e u U t0 ->
-        forall (V : term) s2 (t1 : U :: e |- V : Srt s2),
-        P (U :: e) V (Srt s2) t1 ->
-        forall v (t2 : e |- v : subst u V),
-        P e v (subst u V) t2 ->
-        forall s3 (s : sum_sort s1 s2 s3),
-        P e (Pair (Sum U V) u v) (Sum U V) (type_pair t t0 t1 t2 s)) ->
-       (forall (e : env) T s1 (t : e |- T : Srt s1),
-        P e T (Srt s1) t ->
-        forall (U : term) s2 (t0 : T :: e |- U : Srt s2),
-        P (T :: e) U (Srt s2) t0 -> P e (Prod T U) (Srt s2) (type_prod t t0)) ->
-       (forall (e : env) T s1 (t : e |- T : Srt s1),
-        P e T (Srt s1) t ->
-        forall (U : term) s2 (t0 : T :: e |- U : Srt s2),
-        P (T :: e) U (Srt s2) t0 ->
-        forall s3 (s : sum_sort s1 s2 s3),
-        P e (Sum T U) (Srt s3) (type_sum t t0 s)) ->
-       (forall (e : env) T (t : e |- T : Srt set),
-        P e T (Srt set) t ->
-        forall (U : term) (t0 : T :: e |- U : Srt prop),
-        P (T :: e) U (Srt prop) t0 ->
-        P e (Subset T U) (Srt set) (type_subset t t0)) ->
-       (forall (e : env) t (U V : term) (t0 : e |- t : Sum U V),
-        P e t (Sum U V) t0 -> P e (Pi1 t) U (type_pi1 t0)) ->
-       (forall (e : env) t (U V : term) (t0 : e |- t : Sum U V),
-        P e t (Sum U V) t0 -> P e (Pi2 t) (subst (Pi1 t) V) (type_pi2 t0)) ->
-       (forall (e : env) t (U V : term) (t0 : e |- t : U),
-        P e t U t0 ->
-        forall s (c : e |- U >> V : s),
-        P0 e U V s c -> P e t V (type_conv t0 c)) ->
-       (forall (e : env) A s (t : e |- A : Srt s),
-        P e A (Srt s) t -> P0 e A A s (coerce_refl t)) ->
-       (forall (e : env) A B A' B' s (c : e |- A' >> A : s),
-        P0 e A' A s c ->
-        forall t : e |- A' : Srt s,
-        P e A' (Srt s) t ->
-        forall t0 : e |- A : Srt s,
-        P e A (Srt s) t0 ->
-        forall s' (c0 : A' :: e |- B >> B' : s'),
-        P0 (A' :: e) B B' s' c0 ->
-        forall t1 : A :: e |- B : Srt s',
-        P (A :: e) B (Srt s') t1 ->
-        forall t2 : A' :: e |- B' : Srt s',
-        P (A' :: e) B' (Srt s') t2 ->
-        P0 e (Prod A B) (Prod A' B') s' (coerce_prod c t t0 c0 t1 t2)) ->
-       (forall (e : env) A B A' B' s (c : e |- A >> A' : s),
-        P0 e A A' s c ->
-        forall t : e |- A' : Srt s,
-        P e A' (Srt s) t ->
-        forall t0 : e |- A : Srt s,
-        P e A (Srt s) t0 ->
-        forall s' (c0 : A :: e |- B >> B' : s'),
-        P0 (A :: e) B B' s' c0 ->
-        forall t1 : A :: e |- B : Srt s',
-        P (A :: e) B (Srt s') t1 ->
-        forall t2 : A' :: e |- B' : Srt s',
-        P (A' :: e) B' (Srt s') t2 ->
-        forall s'' (s0 s1 : sum_sort s s' s''),
-        P0 e (Sum A B) (Sum A' B') s'' (coerce_sum c t t0 c0 t1 t2 s0 s1)) ->
-       (forall (e : env) (U P3 U' : term) (c : e |- U >> U' : set),
-        P0 e U U' set c ->
-        forall t : e |- U : Srt set,
-        P e U (Srt set) t ->
-        forall t0 : e |- U' : Srt set,
-        P e U' (Srt set) t0 ->
-        forall t1 : U :: e |- P3 : Srt prop,
-        P (U :: e) P3 (Srt prop) t1 ->
-        P0 e (Subset U P3) U' set (coerce_sub_l c t t0 t1)) ->
-       (forall (e : env) (U U' P3 : term) (c : e |- U >> U' : set),
-        P0 e U U' set c ->
-        forall t : e |- U : Srt set,
-        P e U (Srt set) t ->
-        forall t0 : e |- U' : Srt set,
-        P e U' (Srt set) t0 ->
-        forall t1 : U' :: e |- P3 : Srt prop,
-        P (U' :: e) P3 (Srt prop) t1 ->
-        P0 e U (Subset U' P3) set (coerce_sub_r c t t0 t1)) ->
-       (forall (e : env) A B (C D : term) s (j : e |- A = B : Srt s),
-        P1 e A B (Srt s) j ->
-        forall c : e |- B >> C : s,
-        P0 e B C s c ->
-        forall j0 : e |- C = D : Srt s,
-        P1 e C D (Srt s) j0 -> P0 e A D s (coerce_conv j c j0)) ->
-       (forall (e : env) (U V U' V' : term) s1 s2 (j : e |- U = U' : Srt s1),
-        P1 e U U' (Srt s1) j ->
-        forall j0 : U :: e |- V = V' : Srt s2,
-        P1 (U :: e) V V' (Srt s2) j0 ->
-        P1 e (Prod U V) (Prod U' V') (Srt s2) (jeq_prod j j0)) ->
-       (forall (e : env) A A' s1 (j : e |- A = A' : Srt s1),
-        P1 e A A' (Srt s1) j ->
-        forall B s2 (t : A :: e |- B : Srt s2),
-        P (A :: e) B (Srt s2) t ->
-        forall M M' (j0 : A :: e |- M = M' : B),
-        P1 (A :: e) M M' B j0 ->
-        P1 e (Abs A M) (Abs A' M') (Prod A B) (jeq_abs j t j0)) ->
-       (forall (e : env) A B M M' (j : e |- M = M' : Prod A B),
-        P1 e M M' (Prod A B) j ->
-        forall N N' (j0 : e |- N = N' : A),
-        P1 e N N' A j0 ->
-        P1 e (App M N) (App M' N') (subst N B) (jeq_app j j0)) ->
-       (forall (e : env) A s1 (t : e |- A : Srt s1),
-        P e A (Srt s1) t ->
-        forall B s2 (t0 : A :: e |- B : Srt s2),
-        P (A :: e) B (Srt s2) t0 ->
-        forall M (t1 : A :: e |- M : B),
-        P (A :: e) M B t1 ->
-        forall N (t2 : e |- N : A),
-        P e N A t2 ->
-        P1 e (App (Abs A M) N) (subst N M) (subst N B) (jeq_beta t t0 t1 t2)) ->
-       (forall (e : env) M N A (j : e |- M = N : A),
-        P1 e M N A j ->
-        forall B s (j0 : e |- A = B : Srt s),
-        P1 e A B (Srt s) j0 -> P1 e M N B (jeq_red j j0)) ->
-       (forall (e : env) M N B (j : e |- M = N : B),
-        P1 e M N B j ->
-        forall A s (j0 : e |- A = B : Srt s),
-        P1 e A B (Srt s) j0 -> P1 e M N A (jeq_exp j j0)) ->
-       (forall (e : env) A A' s1 (j : e |- A = A' : Srt s1),
-        P1 e A A' (Srt s1) j ->
-        forall B B' s2 (j0 : A :: e |- B = B' : Srt s2),
-        P1 (A :: e) B B' (Srt s2) j0 ->
-        forall s3 (s : sum_sort s1 s2 s3),
-        P1 e (Sum A B) (Sum A' B') (Srt s3) (jeq_sum j j0 s)) ->
-       (forall (e : env) A A' s1 (j : e |- A = A' : Srt s1),
-        P1 e A A' (Srt s1) j ->
-        forall B B' s2 (j0 : A :: e |- B = B' : Srt s2),
-        P1 (A :: e) B B' (Srt s2) j0 ->
-        forall s3 (s : sum_sort s1 s2 s3) t t' (j1 : e |- t = t' : Sum A B),
-        P1 e t t' (Sum A B) j1 -> P1 e (Pi1 t) (Pi1 t') A (jeq_pi1 j j0 s j1)) ->
-       (forall (e : env) A A' s1 (j : e |- A = A' : Srt s1),
-        P1 e A A' (Srt s1) j ->
-        forall B B' s2 (j0 : A :: e |- B = B' : Srt s2),
-        P1 (A :: e) B B' (Srt s2) j0 ->
-        forall s3 (s : sum_sort s1 s2 s3) u u' v v'
-          (j1 : e |- Pair (Sum A B) u v = Pair (Sum A' B') u' v' : Sum A B),
-        P1 e (Pair (Sum A B) u v) (Pair (Sum A' B') u' v') (Sum A B) j1 ->
-        P1 e (Pi1 (Pair (Sum A B) u v)) u A (jeq_pi1_red j j0 s j1)) ->
-       (forall (e : env) A A' s1 (j : e |- A = A' : Srt s1),
-        P1 e A A' (Srt s1) j ->
-        forall B B' s2 (j0 : A :: e |- B = B' : Srt s2),
-        P1 (A :: e) B B' (Srt s2) j0 ->
-        forall s3 (s : sum_sort s1 s2 s3) t t' (j1 : e |- t = t' : Sum A B),
-        P1 e t t' (Sum A B) j1 ->
-        P1 e (Pi2 t) (Pi2 t') (subst (Pi1 t) B) (jeq_pi2 j j0 s j1)) ->
-       (forall (e : env) A A' s1 (j : e |- A = A' : Srt s1),
-        P1 e A A' (Srt s1) j ->
-        forall B B' s2 (j0 : A :: e |- B = B' : Srt s2),
-        P1 (A :: e) B B' (Srt s2) j0 ->
-        forall s3 (s : sum_sort s1 s2 s3) u u' v v'
-          (j1 : e |- Pair (Sum A B) u v = Pair (Sum A' B') u' v' : Sum A B),
-        P1 e (Pair (Sum A B) u v) (Pair (Sum A' B') u' v') (Sum A B) j1 ->
-        P1 e (Pi2 (Pair (Sum A B) u v)) v (subst u B) (jeq_pi2_red j j0 s j1)) ->
-       (forall (e : env) A A' (j : e |- A = A' : Srt set),
-        P1 e A A' (Srt set) j ->
-        forall B B' (j0 : A :: e |- B = B' : Srt prop),
-        P1 (A :: e) B B' (Srt prop) j0 ->
-        P1 e (Subset A B) (Subset A' B') (Srt set) (jeq_subset j j0)) ->
-       (forall (e : env) M A (t : e |- M : A),
-        P e M A t -> P1 e M M A (jeq_refl t)) ->
-       (forall (e : env) M N A (j : e |- M = N : A),
-        P1 e M N A j -> P1 e N M A (jeq_sym j)) ->
-       (forall (e : env) M N (P3 : term) A (j : e |- M = N : A),
-        P1 e M N A j ->
-        forall j0 : e |- N = P3 : A,
-        P1 e N P3 A j0 -> P1 e M P3 A (jeq_trans j j0)) ->
-       (forall (e : env) M N A B s (j : e |- M = N : A),
-        P1 e M N A j ->
-        forall j0 : e |- A = B : Srt s,
-        P1 e A B (Srt s) j0 -> P1 e M N B (jeq_conv j j0)) ->
-       P2 nil wf_nil ->
-       (forall (e : env) T s (t : e |- T : Srt s),
-        P e T (Srt s) t -> P2 (T :: e) (wf_var t)) ->
-       (forall (e : env) t t0 (c : e |- t : t0 ), P e t t0 c)
-       /\ (forall (e : env) t t0 s (c : e |- t >> t0 : s), P0 e t t0 s c)
-       /\ (forall (e : env) t t0 T (c : e |- t = t0 : T), P1 e t t0 T c)
-       /\ (forall (e : env) (t1 : wf e), P2 e t1).
-Proof.
-  intros.
-  split.
-  intros ; eapply typ_coerce_wf_jeq_mutind with (P:=P) (P0:=P0) (P1:=P1) (P2:=P2) ; auto ; auto.
-  split ; intros.
-  eapply coerce_typ_wf_jeq_mutind with (P:=P) (P0:=P0) (P1 := P1) (P2:=P2) ; auto ; auto.
-  split ; intros.
-  eapply jeq_typ_wf_coerce_mutind with (P:=P) (P0:=P0) (P1 := P1) (P2:=P2) ; auto ; auto.
-  eapply wf_typ_coerce_jeq_mutind with (P:=P) (P0:=P0) (P1 := P1) (P2:=P2) ; auto ; auto.
-Qed.
-  
-  Lemma type_prop_set :
-   forall s, is_prop s -> forall e, wf e -> typ e (Srt s) (Srt kind).
-simple destruct 1; intros ; rewrite H0.
-apply type_prop; trivial.
-apply type_set; trivial.
-Qed.
-
-
-Lemma typ_free_db : forall e t T, typ e t T -> free_db (length e) t.
-Proof.
-  simple induction 1 ; intros ; auto with coc core arith datatypes.
-  inversion_clear H1.
-  apply db_ref.
-  elim H3; simpl in |- *; intros; auto with coc core arith datatypes.
-Qed.
-
-
-Lemma typ_wf : forall e t T, e |- t : T -> wf e.
-simple induction 1; auto with coc core arith datatypes.
-Qed.
-
-
-  Lemma wf_sort :
-   forall n e f,
-   trunc _ (S n) e f ->
-   wf e -> forall t, item _ t e n -> exists s : sort, f |- t : (Srt s).
-simple induction n.
-do 3 intro.
-inversion_clear H.
-inversion_clear H0.
-intros.
-inversion_clear H0.
-inversion_clear H.
-exists s; auto with coc core arith datatypes.
-
-do 5 intro.
-inversion_clear H0.
-intros.
-inversion_clear H2.
-inversion_clear H0.
-elim H with e0 f t; intros; auto with coc core arith datatypes.
-exists x0; auto with coc core arith datatypes.
-
-apply typ_wf with x (Srt s); auto with coc core arith datatypes.
-Qed.
-
-Lemma left_not_kind : forall G t T, G |- t : T -> t <> Srt kind.
-Proof.
-  induction 1 ; intros ; unfold not ; intros ; try discriminate ; auto with coc.
-Qed.
-
-Lemma coerce_prop_prop : forall e, wf e -> e |- Srt prop >> Srt prop : kind.
-Proof.
-  intros.
-  auto with coc.
-Qed.
-
-Lemma coerce_set_set : forall e, wf e -> e |- Srt set >> Srt set : kind.
-Proof.
-  intros.
-  auto with coc.
-Qed.
-
-Lemma coerce_is_prop : forall e, wf e -> forall s, is_prop s -> e |- Srt s >> Srt s : kind.
-Proof.
-  intros.
-  induction H0 ;
-  rewrite H0 ; auto with coc.
-Qed.
-
-Lemma conv_coerce : forall e T T' s, e |- T' : Srt s -> e |- T = T' : Srt s ->
-  e |- T >> T' : s.
-Proof.
- intros.
- apply coerce_conv with T' T' ; auto with coc.
-Qed.
-
-Hint Resolve coerce_prop_prop coerce_set_set coerce_is_prop : coc.
-Hint Resolve conv_coerce typ_wf left_not_kind : coc.
