proof/JRussell/Substitution.v
@@ -3,7 +3,7 @@ Require Import Lambda.Reduction.
 Require Import Lambda.LiftSubst.
 Require Import Lambda.Env.
 Require Import JRussell.Types.
-Require Import JRussell.Thinning.
+Require Import JRussell.Coercion.
 
 Set Implicit Arguments.
 
@@ -12,126 +12,196 @@ Implicit Type s : sort.
 Implicit Types A B M N T t u v : term.
 Implicit Types e f g : env.
 
-Lemma double_sub_weak : forall g (d : term) t, g |- d : t ->
+Lemma ind_sub_weak : forall g (d : term) t, g |- d : t ->
    (forall e u (U : term), e |- u : U ->
-   forall f n, sub_in_env d t n e f -> wf f -> trunc _ n f g -> 
+   forall f n, sub_in_env d t n e f -> trunc _ n f g -> 
    f |- (subst_rec d u n) : (subst_rec d U n)) /\
-   (forall e T U s, e |- T >> U : s->
-   forall f n, sub_in_env d t n e f -> wf f -> trunc _ n f g -> 
-   f |- (subst_rec d T n) >> (subst_rec d U n) : s).
+   (forall e T U s, e |- T >> U : s ->
+   forall f n, sub_in_env d t n e f -> trunc _ n f g -> 
+   f |- (subst_rec d T n) >> (subst_rec d U n) : s) /\
+   (forall e U V T, e |- U = V : T ->
+   forall f n, sub_in_env d t n e f -> trunc _ n f g -> 
+   f |- (subst_rec d U n) = (subst_rec d V n) : (subst_rec d T n)).
 Proof.
 intros g d t H.
-apply double_typ_coerce_mut with
- (P := fun e u (U : term) => fun H0 : e |- u : U =>
- forall f n,
- sub_in_env d t n e f ->
- wf f -> trunc term n f g -> f |- subst_rec d u n : subst_rec d U n)
- (P0 :=
- fun e T (U : term) s => fun H0 : e |- T >> U : s =>
- forall f n,
- sub_in_env d t n e f ->
- wf f -> trunc term n f g -> f |- subst_rec d T n >> subst_rec d U n : s) ;
+apply typ_coerce_jeq_ind with
+   (P:=fun e u (U : term) => fun H : e |- u : U =>
+   forall f n, sub_in_env d t n e f -> trunc _ n f g -> 
+   f |- (subst_rec d u n) : (subst_rec d U n)) 
+   (P1:=fun e U V T => fun H : e |- U = V : T =>
+   forall f n, sub_in_env d t n e f -> trunc _ n f g -> 
+   f |- (subst_rec d U n) = (subst_rec d V n) : (subst_rec d T n))
+   (P0:=fun e T U s => fun H : e |- T >> U : s =>
+   forall f n, sub_in_env d t n e f -> trunc _ n f g -> 
+   f |- (subst_rec d T n) >> (subst_rec d U n) : s) ;
  simpl in |- *;
- try simpl in IHIH ; 
- try simpl in IHIH0 ; 
- try simpl in IHIH1 ;
- try simpl in IHIH2 ;
- try simpl in IHIH3 ; 
- try simpl in IHIH4 ;
- try simpl in IHIH5 ;
- try simpl in IHIH6 ;
  intros; auto with coc core arith datatypes.
 
-elim (lt_eq_lt_dec n0 n); [ intro Hlt_eq | intro Hlt ].
-elim i.
+inversion H0.
+
+inversion H0.
+
+elim (lt_eq_lt_dec n 0); [ intro Hlt_eq | intro Hlt ].
 elim Hlt_eq; clear Hlt_eq.
-case n; [ intro Hlt | intros n1 Hlt ]; intros.
-inversion_clear Hlt.
+intros.
+assert(False) ; try omega ; contradiction.
+intros.
+rewrite b ; simpl.
+rewrite simpl_subst ; auto with arith.
+rewrite lift0.
+rewrite lift0.
+rewrite b in H2.
+rewrite b in H1.
+inversion H1.
+inversion H2.
+rewrite <- H3 ; assumption.
 
-simpl in |- *.
-rewrite H3.
-rewrite simpl_subst; auto with coc core arith datatypes.
-apply type_var; auto with coc core arith datatypes.
-exists x; auto with coc core arith datatypes.
-apply nth_sub_sup with d t n0 e; auto with coc core arith datatypes.
+inversion H1.
+rewrite <- H3 in Hlt.
+assert(False) ; try omega ; contradiction.
+rewrite commut_lift_subst.
+apply type_var with s.
+apply H0 ; auto.
+rewrite <- H4 in H2.
+rewrite <- H5 in H2.
+inversion H2 ; auto.
 
-intro Heq; intros.
-rewrite H3.
-elim Heq.
-rewrite simpl_subst; auto with coc core arith datatypes.
-replace x with t.
-apply thinning_n with g; auto with coc core arith datatypes.
+inversion H2.
+rewrite simpl_subst ; auto with arith.
+rewrite lift0.
+rewrite simpl_subst ; auto with arith.
+rewrite lift0.
+rewrite <- H5 ; assumption.
 
-apply fun_item with e n; auto with coc core arith datatypes.
-apply nth_sub_eq with d f; auto with coc core arith datatypes.
-elim Heq; auto with coc core arith datatypes.
+rewrite commut_lift_subst.
+rewrite commut_lift_subst.
+rewrite <- H5 in H3.
+rewrite <- H6 in H3.
+inversion H3.
+apply type_weak with s ; auto.
 
-apply type_var; auto with coc core arith datatypes.
-apply nth_sub_inf with t e; auto with coc core arith datatypes.
-
-cut (wf (subst_rec d T n :: f)); intros.
-apply type_abs with s1 s2; auto with coc core arith datatypes.
-
-apply wf_var with s1; auto with coc core arith datatypes.
+apply type_abs with s1 s2 ; auto with coc.
 
 rewrite distr_subst.
-apply type_app with (subst_rec d V n); auto with coc core arith datatypes.
+apply type_app with (subst_rec d V n) ; auto with coc.
 
-apply type_pair with s1 s2 s3 ; auto with coc core arith datatypes.
-apply H2 ; auto with coc.
-apply wf_var with s1 ; auto with coc.
-rewrite <- distr_subst ; auto with coc core arith datatypes.
+apply type_pair with s1 s2 s3 ; auto with coc.
+rewrite <- distr_subst ; auto with coc.
 
-cut (wf (subst_rec d T n :: f)); intros.
-apply type_prod with s1; auto with coc core arith datatypes.
+apply type_prod with s1 ; auto with coc.
 
-apply wf_var with s1; auto with coc core arith datatypes.
+apply type_sum with s1 s2 ; auto with coc.
 
-cut (wf (subst_rec d T n :: f)); intros.
-apply type_sum with s1 s2; auto with coc core arith datatypes.
-apply wf_var with s1; auto with coc core arith datatypes.
-
-cut (wf (subst_rec d T n :: f)); intros.
-apply type_subset; auto with coc core arith datatypes.
-
-apply wf_var with set; auto with coc core arith datatypes.
+apply type_subset ; auto with coc.
 
 apply type_pi1 with (subst_rec d V (S n)) ; auto with coc.
 
 rewrite distr_subst.
 simpl.
 apply type_pi2 with (subst_rec d U n) ; auto with coc.
-(*
-cut (wf (subst_rec d U n :: f)).
-intro ; rewrite distr_subst.
-apply type_let_in with (subst_rec d U n) s1 s2 ; auto with coc core arith datatypes.
-apply wf_var with s1 ; auto with coc core arith datatypes.
-*)
-apply type_conv with (subst_rec d U n) s; auto with coc core arith datatypes.
 
-apply coerce_prod with s; auto with coc core arith datatypes.
+apply type_conv with (subst_rec d U n) s ; auto with coc.
 
-apply H3 ; auto with coc core.
-apply wf_var with s ; auto with coc core.
-apply H4 ; auto with coc core.
-apply wf_var with s ; auto with coc core.
-apply H5 ; auto with coc core.
-apply wf_var with s ; auto with coc core.
+inversion H2.
+rewrite simpl_subst ; auto with arith.
+rewrite simpl_subst ; auto with arith.
+rewrite lift0 ; rewrite lift0.
+rewrite <- H5 ; auto.
+rewrite <- H5 in H3.
+rewrite <- H6 in H3.
+inversion H3.
 
-apply coerce_sum with s s' ; auto with coc core.
-apply H3 ; auto with coc core ; apply wf_var with s ; auto with coc core.
-apply H4 ; auto with coc core ; apply wf_var with s ; auto with coc core.
-apply H5 ; auto with coc core ; apply wf_var with s ; auto with coc core.
+rewrite commut_lift_subst.
+rewrite commut_lift_subst.
+apply coerce_weak with s' ; auto with coc.
 
-apply coerce_sub_l ; auto with coc core.
-apply H1 ; auto with coc core ; apply wf_var with set ; auto with coc core.
-eapply coerce_sort_l ; auto with coc core.
+apply coerce_prod with s ; auto with coc.
 
-apply coerce_sub_r ; auto with coc core.
-apply H1 ; auto with coc core ; apply wf_var with set ; auto with coc core.
-eapply coerce_sort_r ; auto with coc core.
+apply coerce_sum with s s' ; auto with coc.
 
-apply coerce_conv with (subst_rec d B n) (subst_rec d C n); auto with coc core.
+apply coerce_trans with (subst_rec d B n) ; auto with coc.
+
+inversion H2.
+do 3 (rewrite simpl_subst ; auto with arith).
+do 3 rewrite lift0.
+rewrite <- H5 ; auto.
+rewrite <- H5 in H3.
+rewrite <- H6 in H3.
+inversion H3.
+
+do 3 (rewrite commut_lift_subst).
+apply jeq_weak with s ; auto with coc.
+
+apply jeq_prod with s1 ; auto with coc.
+
+apply jeq_abs with s1 s2 ; auto with coc.
+
+rewrite distr_subst.
+apply jeq_app with (subst_rec d A n) ; auto with coc.
+
+rewrite distr_subst.
+rewrite distr_subst.
+apply jeq_beta with s1 s2 ; auto with coc.
+
+apply jeq_red with (subst_rec d A n) s ; auto with coc.
+
+apply jeq_exp with (subst_rec d B n) s ; auto with coc.
+
+apply jeq_sum with s1 s2 ; auto with coc.
+
+apply jeq_pair with s1 s2 s3 ; auto with coc.
+simpl.
+rewrite <- distr_subst.
+apply H3 ; auto with coc.
+
+apply jeq_pi1 with (subst_rec d B (S n)) ; auto with coc.
+
+apply jeq_pi1_red with s1 s2 s3 ; auto with coc.
+rewrite <- distr_subst.
+apply H3 ; auto with coc.
+
+rewrite distr_subst.
+simpl.
+apply jeq_pi2 with (subst_rec d A n) ; auto with coc.
+
+rewrite distr_subst.
+apply jeq_pi2_red with s1 s2 s3; auto with coc.
+rewrite <- distr_subst.
+apply H3 ; auto with coc.
+
+
+apply jeq_subset ; auto with coc.
+
+apply jeq_trans with (subst_rec d N n) ; auto with coc.
+
+apply jeq_conv with (subst_rec d A n) s ; auto with coc.
+Qed.
+
+Lemma typ_sub_weak : forall g (d : term) t, g |- d : t ->
+   forall e u (U : term), e |- u : U ->
+   forall f n, sub_in_env d t n e f -> trunc _ n f g -> 
+   f |- (subst_rec d u n) : (subst_rec d U n).
+Proof.
+  intros g d t H.
+  exact (proj1 (ind_sub_weak H)).
+Qed.
+
+Lemma coerce_sub_weak : forall g (d : term) t, g |- d : t ->
+   forall e T U s, e |- T >> U : s ->
+   forall f n, sub_in_env d t n e f -> trunc _ n f g -> 
+   f |- (subst_rec d T n) >> (subst_rec d U n) : s.
+Proof.
+  intros g d t H.
+  exact (proj1 (proj2 (ind_sub_weak H))).
+Qed.
+
+Lemma jeq_sub_weak : forall g (d : term) t, g |- d : t ->
+   forall e U V T, e |- U = V : T ->
+   forall f n, sub_in_env d t n e f -> trunc _ n f g -> 
+   f |- (subst_rec d U n) = (subst_rec d V n) : (subst_rec d T n).
+Proof.
+  intros g d t H.
+  exact (proj2 (proj2 (ind_sub_weak H))).
 Qed.
 
 Theorem substitution : forall e t u U, (t :: e) |- u : U ->
@@ -139,9 +209,8 @@ Theorem substitution : forall e t u U, (t :: e) |- u : U ->
 Proof.
 intros.
 unfold subst in |- *.
-destruct (double_sub_weak H0). 
-apply H1 with (t :: e); auto with coc core arith datatypes.
-apply typ_wf with d t; auto with coc core arith datatypes.
+destruct (ind_sub_weak H0). 
+apply H1 with (t :: e) ; auto with coc core arith datatypes.
 Qed.
 
 Theorem substitution_coerce : forall e t T (U : term) s,
@@ -150,40 +219,21 @@ Theorem substitution_coerce : forall e t T (U : term) s,
 Proof.
 intros.
 unfold subst in |- *.
-destruct (double_sub_weak H0). 
+destruct (ind_sub_weak H0). 
+destruct H2.
 apply H2 with (t :: e); auto with coc core arith datatypes.
-apply typ_wf with d t; auto with coc core arith datatypes.
 Qed.
 
-Hint Resolve substitution substitution_coerce : coc.
-
-Theorem substitution_coerce_conv_l : forall e t T s,
-  (t :: e) |- T : Srt s ->
-  forall d u, e |- d : t -> e |- u : t -> conv d u -> 
-  e |- (subst d T) >> (subst u T) : s.
+Theorem substitution_jeq : forall e t U V T,
+  (t :: e) |- U = V : T ->
+  forall d, e |- d : t -> e |- (subst d U) = (subst d V) : subst d T.
 Proof.
 intros.
-assert(conv T T) ; auto with coc.
-pose (conv_conv_subst _ _ _ _ 0 H2 H3) ; auto.
-apply conv_coerce ; auto with coc ; try (
-change (Srt s) with (subst d (Srt s)) ;
-apply substitution with t ; auto with coc core) ; try (
-change (Srt s) with (subst u (Srt s)) ;
-apply substitution with t ; auto with coc core).
+unfold subst in |- *.
+destruct (ind_sub_weak H0). 
+destruct H2.
+apply H3 with (t :: e); auto with coc core arith datatypes.
 Qed.
 
-Theorem substitution_coerce_conv_l_n : forall e t T s,
-  (t :: e) |- T : Srt s ->
-  forall d u, e |- d : t -> e |- u : t -> conv d u -> 
-  forall n, e |- (subst d T) >> (subst u T) : s.
-Proof.
-intros.
-assert(conv T T) ; auto with coc.
-pose (conv_conv_subst _ _ _ _ 0 H2 H3) ; auto.
-apply conv_coerce ; auto with coc ; try (
-change (Srt s) with (subst d (Srt s)) ;
-apply substitution with t ; auto with coc core) ; try (
-change (Srt s) with (subst u (Srt s)) ;
-apply substitution with t ; auto with coc core).
-Qed.
+Hint Resolve substitution substitution_coerce substitution_jeq : coc.
 
